parse, serialize u64, low-level (no SLow)

src/lowparse/LowParse.Low.Int.fst
@@ -24,6 +24,14 @@ let read_u32 =
   leaf_reader_ext Aux.read_u32 parse_u32 (fun x -> Unique.parse_u32_unique x)
 
 inline_for_extraction
+let read_u64 =
+  leaf_reader_ext Aux.read_u64 parse_u64 (fun x -> Unique.parse_u64_unique x)
+
+inline_for_extraction
+let read_u64_le =
+  leaf_reader_ext Aux.read_u64_le parse_u64_le (fun x -> Unique.parse_u64_le_unique x)
+
+inline_for_extraction
 let serialize32_u8 : serializer32 serialize_u8 = fun v #rrel #rel b pos ->
   [@inline_let] let _ = Unique.serialize_u8_unique v in
   Aux.serialize32_u8 v b pos
@@ -38,8 +46,22 @@ let serialize32_u32 : serializer32 serialize_u32 = fun v #rrel #rel b pos ->
   [@inline_let] let _ = Unique.serialize_u32_unique v in
   Aux.serialize32_u32 v b pos
 
+inline_for_extraction
+let serialize32_u64 : serializer32 serialize_u64 = fun v #rrel #rel b pos ->
+  [@inline_let] let _ = Unique.serialize_u64_unique v in
+  Aux.serialize32_u64 v b pos
+
+inline_for_extraction
+let serialize32_u64_le : serializer32 serialize_u64_le = fun v #rrel #rel b pos ->
+  [@inline_let] let _ = Unique.serialize_u64_le_unique v in
+  Aux.serialize32_u64_le v b pos
+
 let write_u8 = leaf_writer_strong_of_serializer32 serialize32_u8 ()
 
 let write_u16 = leaf_writer_strong_of_serializer32 serialize32_u16 ()
 
 let write_u32 = leaf_writer_strong_of_serializer32 serialize32_u32 ()
+
+let write_u64 = leaf_writer_strong_of_serializer32 serialize32_u64 ()
+
+let write_u64_le = leaf_writer_strong_of_serializer32 serialize32_u64_le ()
