src/lowparse/LowParse.Spec.Int.Aux.fst
@@ -6,6 +6,7 @@ module E = LowParse.BigEndian
 module U8  = FStar.UInt8
 module U16 = FStar.UInt16
 module U32 = FStar.UInt32
+module U64 = FStar.UInt64
 
 let parse_u8_kind : parser_kind = total_constant_size_parser_kind 1
 
@@ -173,3 +174,256 @@ let serialize_u32 : serializer parse_u32 =
   (fun (x: U32.t) -> E.n_to_be 4ul (U32.v x))
 
 #reset-options
+
+let decode_u64
+  (b: bytes { Seq.length b == 8 } )
+: GTot U64.t
+= E.lemma_be_to_n_is_bounded b;
+  U64.uint_to_t (E.be_to_n b)
+
+#push-options "--max_fuel 9 --initial_fuel 9 --z3rlimit 32"
+
+let decode_u64_eq
+  (b: bytes { Seq.length b == 8 } )
+: Lemma
+  (U64.v (decode_u64 b) ==
+    U8.v (Seq.index b 7) + 256 `FStar.Mul.op_Star` (
+    U8.v (Seq.index b 6) + 256 `FStar.Mul.op_Star` (
+    U8.v (Seq.index b 5) + 256 `FStar.Mul.op_Star` (
+    U8.v (Seq.index b 4) + 256 `FStar.Mul.op_Star` (
+    U8.v (Seq.index b 3) + 256 `FStar.Mul.op_Star` (
+    U8.v (Seq.index b 2) + 256 `FStar.Mul.op_Star` (
+    U8.v (Seq.index b 1) + 256 `FStar.Mul.op_Star` (
+    U8.v (Seq.index b 0)
+  ))))))))
+= assert_norm (pow2 8 == 256);
+  E.lemma_be_to_n_is_bounded b;
+  FStar.Math.Lemmas.pow2_le_compat 64 (8 `FStar.Mul.op_Star` 8)
+
+#pop-options
+
+#set-options "--z3rlimit 16"
+
+let decode_u64_injective'
+  (b1: bytes { Seq.length b1 == 8 } )
+  (b2: bytes { Seq.length b2 == 8 } )
+: Lemma
+  (decode_u64 b1 == decode_u64 b2 ==> Seq.equal b1 b2)
+= if decode_u64 b1 = decode_u64 b2
+  then begin
+    E.lemma_be_to_n_is_bounded b1;
+    E.lemma_be_to_n_is_bounded b2;
+    assert (U64.v (U64.uint_to_t (E.be_to_n b1)) == E.be_to_n b1);
+    assert (U64.v (U64.uint_to_t (E.be_to_n b2)) == E.be_to_n b2);
+    assert (E.be_to_n b1 == E.be_to_n b2);
+    E.be_to_n_inj b1 b2
+  end else ()
+
+#reset-options
+
+let decode_u64_injective () : Lemma
+  (make_total_constant_size_parser_precond 8 U64.t decode_u64)
+= Classical.forall_intro_2 decode_u64_injective'
+
+let parse_u64_kind : parser_kind =
+  total_constant_size_parser_kind 8
+
+let parse_u64: parser parse_u64_kind U64.t =
+  decode_u64_injective ();
+  make_total_constant_size_parser 8 U64.t decode_u64
+
+#set-options "--z3rlimit 16"
+
+let parse_u64_spec
+  (b: bytes)
+: Lemma
+  (requires (Seq.length b >= 8))
+  (ensures (
+    let pp = parse parse_u64 b in
+    Some? pp /\ (
+    let (Some (v, consumed)) = pp in
+    U64.v v == E.be_to_n (Seq.slice b 0 8)
+  )))
+= let pp = parse parse_u64 b in
+  assert (Some? pp);
+  let (Some (v, _)) = pp in
+  let s = Seq.slice b 0 8 in
+  assert (v == decode_u64 s);
+  E.lemma_be_to_n_is_bounded s;
+  ()
+
+#set-options "--z3rlimit 128"
+
+let serialize_u64 : serializer parse_u64 =
+  (fun (x: U64.t) ->
+    E.n_to_be 8ul (U64.v x)
+  )
+
+#reset-options
+
+#push-options "--max_fuel 9 --initial_fuel 9 --z3rlimit 1024"
+
+let serialize_u64_eq
+  (x: U64.t)
+  (i: nat {i < 8 })
+: Lemma
+  (U8.v (Seq.index (serialize serialize_u64 x) i) == (
+    let rem7 = U64.v x % 256 in
+    let div7 = U64.v x / 256 in
+    let rem6 = div7 % 256 in
+    let div6 = div7 / 256 in
+    let rem5 = div6 % 256 in
+    let div5 = div6 / 256 in
+    let rem4 = div5 % 256 in
+    let div4 = div5 / 256 in
+    let rem3 = div4 % 256 in
+    let div3 = div4 / 256 in
+    let rem2 = div3 % 256 in
+    let div2 = div3 / 256 in
+    let rem1 = div2 % 256 in
+    let div1 = div2 / 256 in
+    let rem0 = div1 % 256 in
+    if i = 0
+    then rem0
+    else if i = 1
+    then rem1
+    else if i = 2
+    then rem2
+    else if i = 3
+    then rem3
+    else if i = 4
+    then rem4
+    else if i = 5
+    then rem5
+    else if i = 6
+    then rem6
+    else rem7
+  ))
+= assert_norm (pow2 8 == 256)
+
+#pop-options
+
+let decode_u64_le
+  (b: bytes { Seq.length b == 8 } )
+: GTot U64.t
+= E.lemma_le_to_n_is_bounded b;
+  U64.uint_to_t (E.le_to_n b)
+
+#push-options "--max_fuel 9 --initial_fuel 9 --z3rlimit 32"
+
+let decode_u64_le_eq
+  (b: bytes { Seq.length b == 8 } )
+: Lemma
+  (U64.v (decode_u64_le b) ==
+    U8.v (Seq.index b 0) + 256 `FStar.Mul.op_Star` (
+    U8.v (Seq.index b 1) + 256 `FStar.Mul.op_Star` (
+    U8.v (Seq.index b 2) + 256 `FStar.Mul.op_Star` (
+    U8.v (Seq.index b 3) + 256 `FStar.Mul.op_Star` (
+    U8.v (Seq.index b 4) + 256 `FStar.Mul.op_Star` (
+    U8.v (Seq.index b 5) + 256 `FStar.Mul.op_Star` (
+    U8.v (Seq.index b 6) + 256 `FStar.Mul.op_Star` (
+    U8.v (Seq.index b 7)
+  ))))))))
+= assert_norm (pow2 8 == 256);
+  E.lemma_le_to_n_is_bounded b;
+  FStar.Math.Lemmas.pow2_le_compat 64 (8 `FStar.Mul.op_Star` 8)
+
+#pop-options
+
+#set-options "--z3rlimit 16"
+
+let decode_u64_le_injective'
+  (b1: bytes { Seq.length b1 == 8 } )
+  (b2: bytes { Seq.length b2 == 8 } )
+: Lemma
+  (decode_u64_le b1 == decode_u64_le b2 ==> Seq.equal b1 b2)
+= if decode_u64_le b1 = decode_u64_le b2
+  then begin
+    E.lemma_le_to_n_is_bounded b1;
+    E.lemma_le_to_n_is_bounded b2;
+    assert (U64.v (U64.uint_to_t (E.le_to_n b1)) == E.le_to_n b1);
+    assert (U64.v (U64.uint_to_t (E.le_to_n b2)) == E.le_to_n b2);
+    assert (E.le_to_n b1 == E.le_to_n b2);
+    E.le_to_n_inj b1 b2
+  end else ()
+
+#reset-options
+
+let decode_u64_le_injective () : Lemma
+  (make_total_constant_size_parser_precond 8 U64.t decode_u64_le)
+= Classical.forall_intro_2 decode_u64_le_injective'
+
+let parse_u64_le: parser parse_u64_kind U64.t =
+  decode_u64_le_injective ();
+  make_total_constant_size_parser 8 U64.t decode_u64_le
+
+#set-options "--z3rlimit 16"
+
+let parse_u64_le_spec
+  (b: bytes)
+: Lemma
+  (requires (Seq.length b >= 8))
+  (ensures (
+    let pp = parse parse_u64_le b in
+    Some? pp /\ (
+    let (Some (v, consumed)) = pp in
+    U64.v v == E.le_to_n (Seq.slice b 0 8)
+  )))
+= let pp = parse parse_u64_le b in
+  assert (Some? pp);
+  let (Some (v, _)) = pp in
+  let s = Seq.slice b 0 8 in
+  assert (v == decode_u64_le s);
+  E.lemma_le_to_n_is_bounded s;
+  ()
+
+#set-options "--z3rlimit 128"
+
+let serialize_u64_le : serializer parse_u64_le =
+  (fun (x: U64.t) ->
+    E.n_to_le 8ul (U64.v x)
+  )
+
+#reset-options
+
+#push-options "--max_fuel 9 --initial_fuel 9 --z3rlimit 512"
+
+let serialize_u64_le_eq
+  (x: U64.t)
+  (i: nat {i < 8 })
+: Lemma
+  (U8.v (Seq.index (serialize serialize_u64_le x) i) == (
+    let rem0 = U64.v x % 256 in
+    let div0 = U64.v x / 256 in
+    let rem1 = div0 % 256 in
+    let div1 = div0 / 256 in
+    let rem2 = div1 % 256 in
+    let div2 = div1 / 256 in
+    let rem3 = div2 % 256 in
+    let div3 = div2 / 256 in
+    let rem4 = div3 % 256 in
+    let div4 = div3 / 256 in
+    let rem5 = div4 % 256 in
+    let div5 = div4 / 256 in
+    let rem6 = div5 % 256 in
+    let div6 = div5 / 256 in
+    let rem7 = div6 % 256 in
+    if i = 0
+    then rem0
+    else if i = 1
+    then rem1
+    else if i = 2
+    then rem2
+    else if i = 3
+    then rem3
+    else if i = 4
+    then rem4
+    else if i = 5
+    then rem5
+    else if i = 6
+    then rem6
+    else rem7
+  ))
+= assert_norm (pow2 8 == 256)
+
+#pop-options
